pset3/Pset3.v
@@ -1,51 +1,21 @@
-Require Import Frap Pset3Sig.
+Require Import Pset3Sig.
+Require Import List.
+Require Import Frap.
 
-
-Theorem insert_ok: forall tr n, BST tr -> BST (insert n tr).
+Theorem no_extra_children: forall root n1 n2 x,
+  In x (parentsList
+    root
+    (childrenWithNodeName
+         (childrenWithNodeName (cons root nil) n1)
+        n2))
+  -> In x (childrenWithNodeName (cons root nil) n1).
 Proof.
-(*intros n tr.
-simplify.
-case (insert tr n).
-simplify. equality.*)
+  induction root.
+  simplify.
+  equality.
+  simplify.
+  equality.
+  simplify.
 
-
-induct tr.
-simplify.
-propositional.
-simplify.
-cases (compare n t).
-simplify.
-propositional.
-simplify.
-propositional.
-apply IHtr1.
-apply H0.
-simplify.
-apply insert_less_than.
-propositional.
-apply compare_lt_iff.
-apply Heq.
-
-simplify.
-propositional.
-apply IHtr2.
-apply H1.
-apply insert_greater_than.
-propositional.
-apply compare_gt_iff.
-apply Heq.
-Qed.
-
-(* Lemma tree_max: forall tr n, tree_lt (rightmost tr) tr. *)
-
-Lemma rightmost_tree_lt:
-  forall tr v n, tree_lt n tr -> rightmost tr = Some v -> compare v n = Lt.
-Proof.
-  induct tr; simplify.
-  - equality.
-  - cases tr2; simplify; first_order.
-    apply compare_lt_iff.
-    equality.
-Qed.
-
-
+  
+Admitted.
